theories/typing/uniq_alt_borrow.v
@@ -1,0 +1,258 @@
+From lrust.typing Require Export type uniq_alt.
+From lrust.typing Require Import uniq_util typing ptr hints.
+From lrust.util Require Import list.
+Set Default Proof Using "Type".
+
+Open Scope nat.
+
+Implicit Type 𝔄 𝔅: syn_type.
+
+Section uniq_alt_borrow.
+  Context `{!typeG Σ}.
+
+  Lemma alt_type_share_instr {𝔄} p κ (ty : type 𝔄) `{!UniqAlt ty} E L :
+    lctx_lft_alive E L κ →
+    typed_instr E L +[p ◁ (uniq_alt_ty κ ty)] Share (const +[p ◁ &shr{κ} ty])
+      (λ post '-[(a, a')], a' = a -> post -[a]).
+  Proof.
+    iIntros (Hκ ?? [vπ []]) "#LFT #TIME #PROPH #UNIQ #HE $ HL [Huniq _] Hproph".
+    iMod (Hκ with "HE HL") as (q) "[[Htok1 Htok2] Hclose]"; [done..|].
+    iDestruct "Huniq" as (??) "(% & _ & H) /=".
+    iDestruct (ty_uniq_alt_out with "H") as (??->) "[[#? H] [_ Hresolve]]".
+    iDestruct "H" as (?[= ->]??) "([% %Eq] & Hvo & Huniq)"; try lia.
+    iMod (bor_exists_tok with "LFT Huniq Htok1") as (vπ'') "[Huniq Htok1]"; [done|].
+    iMod (bor_exists_tok with "LFT Huniq Htok1") as (d'') "[Huniq Htok1]"; [done|].
+    iMod (bor_acc with "LFT Huniq Htok1") as "[(>#Hd'' & Hpc & Hown) Hclose']"; [done|].
+    iDestruct "Hown" as (?) "[H↦ Hown]".
+    iDestruct ("Hresolve" with "LFT PROPH Htok2 Hown") as "mod".
+    iMod (fupd_mask_mono with "mod") as "(Hresolve&Htok2&Hown)"; [solve_ndisj|].
+    iDestruct (ty.(ty_own_proph) with "LFT [$] Hown [$Htok2]") as "H"; [solve_ndisj|].
+    wp_bind Skip.
+    iApply (wp_step_fupdN_persistent_time_receipt _ _ ∅ with "TIME Hd'' [H]"); [done..| |].
+    { iApply step_fupdN_with_emp.
+      by iApply (fupd_step_fupdN_fupd_mask_mono with "H"). }
+    wp_seq. iDestruct 1 as (ξl q') "/= (%Hdep & Hdt & Hclose'')".
+    iDestruct (uniq_agree with "Hvo Hpc") as "%Hag"; inversion Hag; subst; clear Hag.
+    iMod (uniq_resolve with "PROPH Hvo Hpc Hdt") as "(Hobs & Hpc & Hdt)"; [done| | ].
+    by eapply ty_proph_weaken.
+    iMod ("Hclose''" with "Hdt") as "[Hown Htok]".
+    iMod ("Hclose'" with "[H↦ Hown Hpc]") as "[Huniq Htok2]".
+    { iFrame "#∗". iExists _. iFrame. }
+    do 2 (iMod (bor_sep with "LFT Huniq") as "[_ Huniq]"; [done|]).
+    iDestruct (ty.(ty_share) with "LFT [$] Huniq Htok") as "Hshr"; [done|].
+    iModIntro. wp_seq.
+    iApply (wp_step_fupdN_persistent_time_receipt _ _ ∅ with "TIME Hd'' [Hshr]");
+      [done..| |].
+    { iApply step_fupdN_with_emp.
+      iApply (fupd_step_fupdN_fupd_mask_mono with "Hshr"); done. }
+    wp_seq. iIntros "[Hshr Htok1]". iMod ("Hclose" with "[$Htok1 $Htok2]") as "$".
+    iExists -[_]. rewrite /= right_id. iCombine "Hobs Hresolve Hproph" as "Hobs". iSplitR "Hobs".
+    - iExists _, _. by iFrame "# % Hshr".
+    - iApply proph_obs_impl; [|done]=>/= π.
+      move: (equal_f Eq π)=>/=. case (vπ' π)=>/= ??<-[<-[? Imp]]. by apply Imp.
+  Qed.
+
+  Lemma alt_type_share {𝔄 𝔅l ℭl 𝔇} p κ (ty: type 𝔄) `{!UniqAlt ty} (T: tctx 𝔅l) (T' : tctx ℭl)
+    trx tr e E L (C: cctx 𝔇) :
+    Closed [] e → tctx_extract_ctx E L +[p ◁ (uniq_alt_ty κ ty)] T T' trx →
+    lctx_lft_alive E L κ →
+    typed_body E L C (p ◁ &shr{κ} ty +:: T') e tr -∗
+    typed_body E L C T (Share;; e) (trx ∘
+      (λ post '((a, a') -:: bl), a' = a → tr post (a -:: bl)))%type.
+  Proof.
+    iIntros (? Extr ?) "?".
+    iApply type_seq; [by eapply alt_type_share_instr|solve_typing| |done].
+    destruct Extr as [Htrx _]=>??. apply Htrx. by case.
+  Qed.
+
+  Lemma uniq_alt_ty_eq_shr {𝔄} κ' κ (ty: type 𝔄) `{!UniqAlt ty} E L: 
+    eqtype E L (&shr{κ'} (&uniq{κ} ty)) (&shr{κ'} (uniq_alt_ty κ ty)) id id.
+  Proof. apply equiv_eqtype. done. Qed.
+
+  Lemma alt_type_deref_shr_uniq {𝔄 𝔅l ℭl 𝔇} κ κ' x p e (ty: type 𝔄) `{!UniqAlt ty}
+    (T: tctx 𝔅l) (T': tctx ℭl) trx tr E L (C: cctx 𝔇) :
+    Closed (x :b: []) e →
+    tctx_extract_ctx E L +[p ◁ &shr{κ} (uniq_alt_ty κ' ty)] T T' trx →
+    lctx_lft_alive E L κ → lctx_lft_incl E L κ κ' →
+    (∀v: val, typed_body E L C (v ◁ &shr{κ} ty +:: T') (subst' x v e) tr) -∗
+    typed_body E L C T (let: x := !p in e)
+      (trx ∘ (λ post '((a, _) -:: bl), tr post (a -:: bl))).
+  Proof.
+    iIntros. iApply (type_deref_shr_uniq κ κ' x p e ty); [|done|done|done].
+    eapply tctx_incl_trans. exact H0. eapply tctx_incl_ext. eapply subtype_tctx_incl. apply uniq_alt_ty_eq_shr.
+    intros ?[??]. simpl. done.
+  Qed.
+
+  Lemma alt_tctx_reborrow_uniq {𝔄} E L p (ty: type 𝔄) `{!UniqAlt ty} κ κ' :
+    lctx_lft_incl E L κ' κ →
+    tctx_incl E L +[p ◁ uniq_alt_ty κ ty] +[p ◁ &uniq{κ'} ty; p ◁{κ'} uniq_alt_ty κ ty] 
+      (λ post '-[(a, a')], ∀a'': 𝔄, post -[(a, a''); (a'', a')]).
+  Proof.
+    intros κκ'. split; [intros ??? [[??][]]; by apply forall_proper|].
+    iIntros (??[vπ[]]?) "#LFT #PROPH #UNIQ E L [(%&%&%&⧖&uniq) _] Obs".
+    have ?: Inhabited 𝔄 := populate (vπ inhabitant).1.
+    iDestruct (κκ' with "L E") as "#κ⊑κ'". iFrame "L".
+    iDestruct (ty_uniq_alt_out with "uniq") as (??->) "([#In uniq]&W&_)".
+    iDestruct "uniq" as (?[=->] ? ξi [Le Eq]) "[ξVo ξBor]". set ξ := PrVar _ ξi.
+    move: Le=> /succ_le[?[->?]].
+    iMod (rebor with "LFT κ⊑κ' ξBor") as "[ξBor ToξBor]"; [done|].
+    iMod (uniq_intro (fst ∘ vπ') with "PROPH UNIQ") as (ζi) "(ζVo & ζPc)"; [done|].
+    set ζ := PrVar _ ζi.
+    iMod (bor_create _ κ' (∃vπ' d', .VO[ξ] vπ' d' ∗ ⧖(S d') ∗ .PC[ζ, ty.(ty_proph)] vπ' d')%I
+      with "LFT [⧖ ξVo ζPc]") as "[ζBor ToζBig]"; [done| |].
+    { iExists _, _. iFrame "ξVo ζPc". iApply persistent_time_receipt_mono; [|done]. lia. }
+    iMod (bor_combine with "LFT ξBor ζBor") as "Bor"; [done|].
+    iExists -[λ π, ((vπ' π).1, π ζ); λ π, (π ζ, f (vπ' π).2)]. iSplitR "Obs"; last first.
+    { iApply (proph_obs_impl with "Obs") => /= π. case (vπ' π)=>/= ?? All. apply All. }
+    iMod (bor_acc_atomic_cons with "LFT Bor") as
+      "[[[ξBig ζBig] ToBor]|[#†κ' TolftN]]"; [done| |]; last first.
+    { iMod "TolftN" as "_". iMod ("ToξBor" with "†κ'").
+      iMod ("ToζBig" with "†κ'") as (??) "(>ξVo & >#⧖ & ζPc)".
+      iMod (uniq_strip_later with "ζVo ζPc") as (<-<-) "[ζVo ζPc]". iSplitL "ζVo".
+      - iExists _, _. iFrame "⧖". iSplitR; [done|].
+        iSplitR; [by iApply lft_incl_trans|]. iExists _, ζi. iFrame "ζVo".
+        iSplitR; [done|]. by iApply bor_fake.
+      - iModIntro. iSplitL; [|done]. iExists _. iSplit; [done|]. iIntros "_!>".
+        iExists _, _. iFrame "⧖". iSplitL "ζPc"; last first.
+        { iApply "W". iFrame "In". iExists _, _. by iFrame. }
+        iNext. iDestruct (proph_ctrl_eqz' with "PROPH ζPc") as "Eqz".
+        simpl. iApply proph_eqz_mono; last first.
+        iApply ((proph_eqz_prod _ _ _) with "[Eqz]"); [done|iApply (proph_eqz_refl _ (λ vπ ξl, vπ ./[𝔄] ξl))].
+        simpl. intros ? (?&?&->&?&?). eexists _, _. done.  }
+    iDestruct "ξBig" as (??) "(>#⧖ & ξPc & ↦ty)".
+    iDestruct "ζBig" as (??) "(>ξVo & _ & ζPc)".
+    iMod (uniq_strip_later with "ξVo ξPc") as (<-<-) "[ξVo ξPc]".
+    iMod (uniq_strip_later with "ζVo ζPc") as (<-<-) "[ζVo ζPc]".
+    iMod ("ToBor" $! (∃ vπ' d', ⧖(S d') ∗ .PC[ζ, ty.(ty_proph)] vπ' d' ∗
+      l ↦∗: ty.(ty_own) vπ' d' tid)%I with "[ξVo ξPc] [ζPc ↦ty]") as "ζBor".
+    { iIntros "!> (%&% & #? & ζPc & ↦ty)".
+      iMod (uniq_update with "UNIQ ξVo ξPc") as "[ξVo ξPc]"; [solve_ndisj|].
+      iSplitL "↦ty ξPc"; iExists _, _; by iFrame. }
+    { iNext. iExists _, _. by iFrame. }
+    iModIntro. iSplitL "ζVo ζBor"; [|iSplitL; [|done]].
+    { iExists _, _. iSplit; [done|]. iFrame "⧖".
+      iSplitR; [by iApply lft_incl_trans|]. iExists _, _. by iFrame. }
+    iExists _. iSplit; [done|]. iIntros "#†κ'". iMod ("ToξBor" with "†κ'") as "ξBor".
+    iMod ("ToζBig" with "†κ'") as (vπ'' ?) "(>ξVo & >⧖' & ζPc)". iModIntro.
+    iExists _, _. iFrame "⧖'". iSplitL "ζPc".
+    - iNext. iDestruct (proph_ctrl_eqz' with "PROPH ζPc") as "Eqz".
+      iApply proph_eqz_mono; last first.
+      iApply (proph_eqz_prod _ (pair ∘ vπ'' ⊛ (f ∘ snd ∘ vπ')) with "[Eqz]");
+      [done|iApply (proph_eqz_refl _ (λ vπ ξl, vπ ./[𝔄] ξl))].
+      simpl. intros ?(?&?&->&?&?). eexists _, _. done.
+    - iApply ("W" $! (pair ∘ vπ'' ⊛ (snd ∘ vπ'))). iFrame "In". iExists _, _.
+      rewrite /uniq_body (proof_irrel (prval_to_inh _) (prval_to_inh (fst ∘ vπ'))).
+      by iFrame.
+  Qed.
+
+  Lemma tctx_extract_hasty_reborrow {𝔄 𝔅l} (ty ty': type 𝔄) `{!UniqAlt ty'} κ κ' (T: tctx 𝔅l) E L p :
+    lctx_lft_incl E L κ' κ → eqtype E L ty ty' id id →
+    tctx_extract_elt E L (p ◁ &uniq{κ'} ty) (p ◁ (uniq_alt_ty κ ty') +:: T)
+      (p ◁{κ'} (uniq_alt_ty κ ty') +:: T) (λ post '((a, a') -:: bl),
+        ∀a'': 𝔄, post ((a, a'') -:: (a'', a') -:: bl)).
+  Proof.
+    move=> ??. eapply tctx_incl_impl.
+    - apply (tctx_incl_frame_r +[_] +[_;_]).
+      eapply tctx_incl_trans; [by apply alt_tctx_reborrow_uniq|].
+      by apply subtype_tctx_incl, uniq_subtype, eqtype_symm.
+    - by move=>/= ?[[??]?].
+    - intros ??? [[??]?]. by apply forall_proper.
+  Qed.
+
+  Lemma alt_type_deref_uniq_uniq_instr {𝔄 E L} κ κ' p (ty : type 𝔄) `{!UniqAlt ty} :
+    lctx_lft_alive E L κ →
+    typed_instr_ty E L +[p ◁ &uniq{κ} (uniq_alt_ty κ' ty)] (!p) (&uniq{κ} ty)
+      (λ post '-[((v, w), (v', w'))], w' = w → post (v, v')).
+  Proof.
+    iIntros (Hκ tid ? [vπ []]) "/= #LFT #TIME #PROPH #UNIQ #HE $ HL [Hp _] Hproph".
+    iMod (Hκ with "HE HL") as (q) "[Htok Hclose]"; first solve_ndisj.
+    wp_apply (wp_hasty with "Hp").
+    iIntros ([[]|] [|depth1]) "% #Hdepth1 [#Hκκ' H] //=";
+      iDestruct "H" as (d' ξi) "([% %vπEqξ] & ξVo & Huniq)"; first lia.
+    move: vπEqξ. set ξ := PrVar _ ξi=> vπEqξ.
+    iAssert (κ ⊑ foldr meet static (ty_lfts ty))%I as "Hκ".
+    { iApply lft_incl_trans; [done|]. iApply lft_intersect_incl_r. }
+    iMod (bor_acc_cons with "LFT Huniq Htok") as "[big Hclose']"; [done|].
+    iMod (bi.later_exist_except_0 with "big") as (? depth2) "(>#Hdepth2' & ξPc & (%&>Hl&uniq))".
+    have ?: Inhabited 𝔄 := populate (vπ inhabitant).1.1.
+    iDestruct (ty_uniq_alt_out with "uniq") as "(%&%&>->&(#Hκ'&%&>->&%&%ωi&>[% %ωEq]&ωVo & Hbor)&Halt&_)".
+    case depth2 as [|depth2]; [lia|]. set ω := PrVar _ ωi.
+    iMod (uniq_strip_later with "ξVo ξPc") as (fstEq->) "[ξVo ξPc]".
+    iMod (uniq_update ξ with "UNIQ ξVo ξPc") as "[ξVo ξPc]"; [done|].
+    iMod ("Hclose'" $! (∃l': loc, l ↦∗ [ #l' ] ∗
+      (∃ vπ' d', .VO[ω] vπ' d' ∗ .PC[ξ, _] (prod_map id f ∘ (λ π, (vπ' π, (π ω)))) (S d') ∗ ⧖ (S (S d'))) ∗
+      &{κ'}(∃ vπ' d', ⧖(S d') ∗ .PC[ω, ty.(ty_proph)] vπ' d' ∗ l' ↦∗: ty.(ty_own) vπ' d' tid))%I
+      with "[Halt] [Hbor Hl ωVo ξPc]") as "[Hbor Htok]".
+    { iIntros "!> H !>!>". iDestruct "H" as (l') "(H↦ & (%&%& ωVo & ξPc & ⧖) & H)".
+      iExists _, (S d'). iFrame "⧖ ξPc". iExists _. iFrame "H↦".
+      iApply "Halt". iFrame "Hκ'". iExists d', ωi. rewrite /uniq_body.
+      rewrite (proof_irrel (prval_to_inh _) (prval_to_inh (fst ∘ vπ'))).
+      by iFrame. }
+    { iNext. iExists _. iFrame "Hl Hbor". iExists _, _. iFrame.
+      iApply (persistent_time_receipt_mono); [|done]. lia. }
+    iClear "Hdepth1 Hdepth2'". clear dependent p depth1 Hκ.
+    iMod (bor_exists with "LFT Hbor") as (l') "Hbor"; [done|].
+    iMod (bor_sep with "LFT Hbor") as "[H↦ Hbor]"; [done|].
+    iMod (bor_acc with "LFT H↦ Htok") as "[>H↦ Hclose']"; [done|].
+    iMod (bor_sep with "LFT Hbor") as "[BorVoPc Hbor]"; [done|].
+    iMod (bor_unnest with "LFT Hbor") as "Hbor"; [done|].
+    rewrite heap_mapsto_vec_singleton.
+    iApply wp_fupd. iApply wp_cumulative_time_receipt=>//. wp_read. iIntros "Ht".
+    iMod "Hbor". iMod ("Hclose'" with "[H↦]") as "[_ Htok]"; first by auto.
+    iMod (bor_combine with "LFT BorVoPc [Hbor]") as "Hbor"; [done| |].
+    { iApply (bor_shorten with "[] Hbor").
+      iApply lft_incl_glb; [|iApply lft_incl_refl].
+      iApply lft_incl_trans; [iApply "Hκκ'" |]. iApply lft_intersect_incl_l. }
+    iMod (bor_acc_cons with "LFT Hbor Htok") as "[[VoPc Hown] Hclose']"; [done|].
+    iDestruct "VoPc" as (vπ'' ?) "(Hvo & Hpc & ?)".
+    iMod (bi.later_exist_except_0 with "Hown") as (wπ depth3') "(>#? & Hpcω & Hown)".
+    iMod (uniq_strip_later with "ξVo Hpc") as (?->) "[ξVo ξPc]".
+    have ->: vπ'' = fst ∘ vπ'.
+    (* TODO: remove usage of fun_ext here.  *)
+    { fun_ext => x /=. move: (equal_f H x) => /= y. by inversion y.  }
+    iMod (uniq_strip_later with "Hvo Hpcω") as (<-->) "[ωVo ωPc]".
+    iMod (uniq_intro (fst ∘ (fst ∘ vπ)) with "PROPH UNIQ") as (ζi) "[ζVo ζPc]"; [done|].
+    set ζ := PrVar _ ζi.
+    iDestruct (uniq_proph_tok with "ζVo ζPc") as "(ζVo & ζ & ToζPc)".
+    iDestruct (uniq_proph_tok with "ωVo ωPc") as "(ωVo & ω & ToωPc)".
+    iMod (uniq_preresolve ξ [ζ; ω] (prod_map id f ∘ (λ (π: proph_asn), (π ζ, π ω))) with "PROPH ξVo ξPc [$ζ $ω]")
+      as "(Hobs & (ζ & ω &_) & Heqz)"; [done| |done|].
+    { apply proph_dep_constr; apply (proph_dep_prod [_] [_]); apply proph_dep_one. }
+    iDestruct ("ToζPc" with "ζ") as "ζPc".
+    iDestruct ("ToωPc" with "ω") as "ωPc".
+    iMod ("Hclose'" $! (∃vπ' d', ⧖ (S d') ∗ .PC[ζ, ty.(ty_proph)] vπ' d' ∗
+      l' ↦∗: ty.(ty_own) vπ' d' tid)%I with "[Heqz ωVo ωPc Ht] [Hown ζPc]") as "[? Htok]".
+    { iIntros "!> H".
+      iMod (bi.later_exist_except_0 with "H") as (? ?) "(>#Hd' & Hpc & Hinner)".
+      iMod (uniq_update with "UNIQ ωVo ωPc") as "[ωVo ωPc]"; [solve_ndisj|].
+      iSplitR "Hinner ωPc".
+      - iExists _, d'.
+        iMod (cumulative_persistent_time_receipt with "TIME Ht Hd'") as "$";
+          [solve_ndisj|].
+        iFrame. iApply "Heqz". iDestruct (proph_ctrl_eqz' with "PROPH Hpc") as "Eqz".
+        iApply proph_eqz_mono; last first.
+        iApply (proph_eqz_constr2 with "Eqz []"). iApply (proph_eqz_refl _ (λ vπ ξl, vπ ./[𝔄] ξl)).
+        simpl. intros ? (?&?&->&?&?). eexists a, _, _, _. split. done. split. fun_ext=>?/=. done. done.
+      - iExists _, _. by iFrame. }
+    { iExists _, _. iFrame. rewrite fstEq. by iFrame. }
+    iExists -[λ π, ((vπ π).1.1 , π ζ)]. rewrite right_id.
+    iMod ("Hclose" with "Htok") as "$". iSplitR "Hproph Hobs".
+    - iExists _, _. iFrame "#". iSplitR; [done|]. iExists _, ζi. by iFrame.
+    - iCombine "Hproph Hobs" as "?". iApply proph_obs_impl; [|done]=>/= π.
+      move: (equal_f vπEqξ π) (equal_f ωEq π) (equal_f fstEq π)=>/=. case (vπ π)=> [[??][??]]/=.
+      case (π ξ)=> ??[=<-<-<-][=->->][Imp[=<-?]]. by apply Imp.
+  Qed.
+
+  Lemma alt_type_deref_uniq_uniq {𝔄 𝔅l ℭl 𝔇} κ κ' x p e (ty: type 𝔄) `{!UniqAlt ty}
+    (T: tctx 𝔅l) (T': tctx ℭl) trx tr E L (C: cctx 𝔇) :
+    Closed (x :b: []) e →
+    tctx_extract_ctx E L +[p ◁ &uniq{κ} (uniq_alt_ty κ' ty)] T T' trx →
+    lctx_lft_alive E L κ → lctx_lft_incl E L κ κ' →
+    (∀v: val, typed_body E L C (v ◁ &uniq{κ} ty +:: T') (subst' x v e) tr) -∗
+    typed_body E L C T (let: x := !p in e) (trx ∘
+      (λ post '(((v, w), (v', w')) -:: cl), w' = w → tr post ((v, v') -:: cl)))%type.
+  Proof.
+    iIntros. iApply typed_body_tctx_incl; [done|].
+    by iApply type_let; [by eapply alt_type_deref_uniq_uniq_instr|solve_typing| |done].
+  Qed.
+End uniq_alt_borrow.
